src/Bitstream.v
@@ -1,0 +1,21 @@
+
+Require Import AST.
+
+(* any finite bitstream *)
+(* use to state correctness of crypto functions *)
+Inductive finite_bitstream : list val -> Prop :=
+| empty_stream :
+    finite_bitstream nil
+| one_more :
+    forall b l,
+      finite_bitstream l ->
+      finite_bitstream (bit b :: l).
+
+(* bits with length encoded *)
+Inductive n_bits : nat -> list val -> Prop :=
+| empty_bits :
+    n_bits O nil
+| another_bit :
+    forall n l b,
+      n_bits n l ->
+      n_bits (S n) (bit b :: l).
