src/EvalTac.v
@@ -25,6 +25,7 @@ Ltac init_globals global_env :=
   assert (Htrue : global_env (9, "True") = Some (mb 0 0 true_builtin)) by reflexivity;
   assert (Hfalse : global_env (10, "False") = Some (mb 0 0 false_builtin)) by reflexivity;
   assert (Hgt : global_env (14,">") = Some (mb 1 2 Gt)) by reflexivity;
+  assert (Hxor : global_env (28,"^") = Some (mb 1 2 Xor)) by reflexivity;
   assert (Hat : global_env (40, "@") = Some (mb 3 2 At)) by reflexivity;
   assert (Hsplit : global_env (37,"split") = Some (mb 3 1 split)) by reflexivity;
   assert (HsplitAt : global_env (35,"splitAt") = Some (mb 3 1 splitAt)) by reflexivity;
