src/HexConvert.v
@@ -1,0 +1,70 @@
+Require Import String.
+
+Require Import Coqlib.
+
+Require Import Utils.
+Import HaskellListNotations.
+Open Scope string.
+
+Require Import Values.
+Require Import AST.
+Require Import Bitvectors.
+
+(* Convert a hex string to a list of bits *)
+Definition hex_digits := match collect [get 0 "0",get 0 "1",get 0 "2",get 0 "3",
+                                        get 0 "4",get 0 "5",get 0 "6",get 0 "7",
+                                        get 0 "8",get 0 "9",get 0 "a",get 0 "b",
+                                        get 0 "c",get 0 "d",get 0 "e",get 0 "f"] with
+                         | Some l => l
+                         | None => nil
+                         end.
+
+Lemma hex_digits_not_nil :
+  hex_digits <> nil.
+Proof.
+  unfold hex_digits. simpl.
+  congruence.
+Qed.
+
+Fixpoint lookup_h {A : Type} (eq_dec : forall (a b : A), {a = b} + {a <> b}) (x : A) (l : list A) : option nat :=
+  match l with
+  | nil => None
+  | f :: r =>
+    if eq_dec f x then Some O else
+      match lookup_h eq_dec x r with
+      | Some n => Some (S n)
+      | None => None
+      end
+  end.
+
+Definition lookup (a : Ascii.ascii) : option nat :=
+  lookup_h Ascii.ascii_dec a hex_digits.
+
+
+Definition to_bits (a : Ascii.ascii) : option (list val) :=
+  match lookup a with
+  | Some n =>
+    Some (@from_bitv 4 (@repr 4 (Z.of_nat n)))
+  | None => None
+  end.
+
+Fixpoint val_of_hex_string (s : string) : option (list val) :=
+  match s with
+  | EmptyString => Some nil
+  | String a s' =>
+    match val_of_hex_string s' with
+    | Some l =>
+      match to_bits a with
+      | Some bs => Some (bs ++ l)%list
+      | None => None
+      end
+    | None => None
+    end
+  end.
+
+
+Definition val_of_hex_lit (s : string) : list val :=
+  match val_of_hex_string (substring 2 (String.length s) s) with
+  | Some l => l
+  | None => nil
+  end.
