verif/Xor_verif.v
@@ -1,0 +1,220 @@
+Require Import List.
+Import ListNotations.
+Require Import String.
+
+(* Borrow from CompCert *)
+Require Import Coqlib.
+Require Import Bitvectors.
+
+Require Import AST.
+Require Import Semantics.
+Require Import Utils.
+Require Import Builtins.
+Require Import BuiltinSem.
+Require Import Values.        
+Require Import Bitstream.
+
+Require Import EvalTac.
+
+Import HaskellListNotations.
+Open Scope string.
+
+Require Import Xor.
+
+(* expects a type variable, but ignores it *)
+Definition decrypt : Expr := (ETApp (EVar (243,"decrypt")) (ETyp (TCon (TC (TCNum 3)) nil))).
+Definition encrypt : Expr := (ETApp (EVar (242,"encrypt")) (ETyp (TCon (TC (TCNum 3)) nil))).
+
+Notation "eval_expr* GE E V" := (eval_expr GE _ E V) (at level 99, only printing).
+Notation "vcons* V EXP" := (vcons V EXP _) (at level 98, only printing).
+Notation "force_list* V VS" := (force_list _ _ V VS) (at level 97, only printing).
+
+Lemma single_bit_roundtrip :
+  forall (b b' : bool),
+    (if (if b then (if b' then false else true) else b') then (if b' then false else true) else b') = b.
+Proof.
+  intros. destruct b; destruct b'; simpl; auto.
+Qed.
+
+
+Lemma xor_roundtrip :
+  forall pt,
+    Forall (n_bits 8%nat) pt ->
+    forall k,
+      n_bits (8%nat) k ->
+      exists ciphertext,
+        eval_expr ge empty (EApp (EApp encrypt (EValue (thunk_list k))) (EList (map EList (map (map EValue) pt))) ) ciphertext /\
+        exists v',
+          eval_expr ge empty (EApp (EApp decrypt (EValue (thunk_list k))) (EValue ciphertext)) v' /\
+          exists vls,
+            force_list ge empty v' vls /\
+            Forall2 (force_list ge empty) vls pt.
+Proof.
+  induction 1; intros;
+    do 9 match goal with
+         | [ H : n_bits _ _ |- _ ] => inversion H
+         end; subst.
+  - clear -H.
+    eexists. split.
+    e. e. e. g.
+    repeat e. 
+    repeat e. repeat e. repeat e.
+    repeat e. repeat e.
+    e. 
+    eapply eval_comp_imp_nil.
+    repeat e. simpl. omega.
+    eexists.  split.
+    e. e. e. g. e. e. e.
+    e. e. e. e. eapply eval_comp. eapply eval_comp_imp_nil.
+    repeat e. simpl. omega.
+
+    eexists. split.
+    e. e.
+    
+  - clear -H1 H H0 IHForall.
+    inversion H. inversion H3. inversion H6. inversion H9. inversion H12.
+    inversion H15. inversion H18. inversion H21. inversion H24. subst.
+    clear -H1 H H0 IHForall.
+    eapply IHForall in H1; eauto.
+    clear IHForall. destruct H1. destruct H1.
+    inversion H1. subst.
+    destruct H2. destruct H2. destruct H3. destruct H3.
+    inversion H7. subst.
+
+    init_globals ge.
+
+    eexists; split.
+    + e. (* run encrypt *)
+      -- e. simpl. e. g.
+         repeat e. repeat e. repeat e. repeat e.
+         repeat e.
+      -- simpl. e. e. e. repeat e. eassumption. (* use part of inductive hypothesis *)
+      -- e. e. e. eapply idx_last. e. e. e. e. e. e. e. e. e. repeat e.
+         e. e. e. e. e.
+         eapply eval_lift_binary_builtin.
+         simpl; auto. simpl. instantiate (3 := (EVar (3,"")) :: nil). reflexivity.
+         e. e. e. eapply eval_binary_over_bit_to_bit. simpl. reflexivity.
+         e. e.
+    +
+Admitted.
+(*      (* BELOW MIGHT BE RIGHT IDK *)
+      eexists; split. (* run decrypt *)
+      e. e. e. g.
+      e. repeat e. e. e. e. e. e. e.
+      e. eapply idx_last. e. e. e. e. e. e. e.
+      e. e. e. repeat e. repeat e.
+      e. e. e. e. e.
+      eapply eval_lift_binary_builtin.
+      simpl. auto.
+      simpl.
+      instantiate (3 := (EVar (3,"")) :: nil). reflexivity.
+      simpl. e. e. e. simpl.
+      eapply eval_binary_over_bit_to_bit. reflexivity. e. e.
+
+      * destruct vs.
+        -- (* encrypt/decrypt exactly one byte, nothing more *)
+          eexists. split.
+          e. eapply eval_comp_imp_nil. e. e. e. e.
+          eapply eval_comp_imp_nil. repeat e. simpl. omega.
+          e. simpl. omega.
+          e. simpl. e.
+          rewrite single_bit_roundtrip. e.
+          e. e. e. e. simpl. eapply eval_binary_over_bit_to_bit. reflexivity.
+          e. e. e. eapply eval_binary_over_bit_to_bit. reflexivity.
+          e. e. simpl.
+          rewrite single_bit_roundtrip. e.
+          e. e. e. e. eapply eval_binary_over_bit_to_bit. reflexivity.
+          e. e. e. eapply eval_binary_over_bit_to_bit. reflexivity.
+          simpl. e. e. simpl.
+          rewrite single_bit_roundtrip. e.
+          e. e. e. e. eapply eval_binary_over_bit_to_bit. reflexivity.
+          e. e. e. eapply eval_binary_over_bit_to_bit. reflexivity.
+          simpl. e. e. simpl.
+          rewrite single_bit_roundtrip. e.
+          e. e. e. e. eapply eval_binary_over_bit_to_bit. reflexivity.
+          e. e. e. eapply eval_binary_over_bit_to_bit. reflexivity.
+          simpl. e. e. simpl.
+          rewrite single_bit_roundtrip. e.
+          e. e. e. e. eapply eval_binary_over_bit_to_bit. reflexivity.
+          e. e. e. eapply eval_binary_over_bit_to_bit. reflexivity.
+          simpl. e. e. simpl.
+          rewrite single_bit_roundtrip. e.
+          e. e. e. e. eapply eval_binary_over_bit_to_bit. reflexivity.
+          e. e. e. eapply eval_binary_over_bit_to_bit. reflexivity.
+          simpl. e. e. simpl.
+          rewrite single_bit_roundtrip. e.
+          e. e. e. e. eapply eval_binary_over_bit_to_bit. reflexivity.
+          e. e. e. eapply eval_binary_over_bit_to_bit. reflexivity.
+          simpl. e. e. simpl.
+          rewrite single_bit_roundtrip. eapply force_cons.
+          eapply eval_lift_binary_nil. eapply eval_lift_binary_nil. e. e. e. e.
+          destruct l; simpl in H8; inversion H8. e.
+        -- (* inductive case, encrypt/decrypt one byte then apply IH *)
+          
+          simpl.
+          
+          destruct l; try solve [simpl in H8; inversion H8].
+          inversion H0. subst. inversion H11. inversion H10.
+          inversion H15. inversion H18. inversion H21.
+          inversion H24. inversion H27. inversion H30. inversion H33. subst.
+          clear H33 H27 H21 H15 H10 H18 H24 H30.
+          simpl in H8. simpl in H7. inversion H8. inversion H7.
+          subst.
+
+          inversion H14. subst.
+          destruct vs0; simpl in H20; try congruence.
+          inversion H20. subst.
+          inversion H10. subst.
+          inversion H21. subst.
+          inversion H23. subst.
+          inversion H25. subst.
+          inversion H27. subst.
+          inversion H29. subst.
+          inversion H31. subst.
+          inversion H33. subst.
+          inversion H35. subst.
+          clear H35.
+          inversion H32. subst.
+          inversion H30. subst.
+          inversion H28. subst.
+          inversion H26. subst.
+          inversion H24. subst.
+          inversion H22. subst.
+          inversion H19. subst.
+          inversion H17. subst.
+          
+          eexists. split.
+
+          eapply force_cons.
+
+          --- 
+            e. e. eapply idx_last. e. e.
+            e. e. e. e. e. e. 
+            e. e.
+            e. e. e. e.
+            e. e. e. repeat e. repeat e. e. e. e. e.
+            eapply eval_lift_binary_builtin. simpl. auto.
+            simpl. instantiate (3 := (EVar (3,""))::nil). reflexivity.
+            e. e. e.
+            eapply eval_binary_over_bit_to_bit.
+            simpl. reflexivity.
+            e. e. e. e. e. e. e. e. e. repeat e.
+            e. e. e. e. e.
+            eapply eval_lift_binary_builtin. simpl. auto.
+            simpl. instantiate (3 := (EVar (3,""))::nil). reflexivity.
+            e. e. e.
+            eapply eval_binary_over_bit_to_bit.
+            simpl. reflexivity.
+            e. e.
+
+          --- (* inductive hypothesis needs to be used here I think *)
+            
+            e. e. e. e. e. e. e. e. e. e. e. e.
+            e. e. e. e. e. e. e. e. e. e. e. e. e. e. e. e.
+            e. eapply eval_lift_binary_builtin.
+            e. simpl. instantiate (3 := (EVar (3,""))::nil). reflexivity.
+            e. e. e. eapply eval_binary_over_bit_to_bit. reflexivity.
+            e. e. e.
+            (* HERE *)
+            (* What are the useful hypotheses? *)
+            *)
